fix more proofs

lib/Checksums/F2_X_Lemmas.i.dfy
@@ -161,7 +161,7 @@ module F2_X_Lemmas {
     }
   }
 
-  function set_digit(p: Bits, q: Bits, i: nat) : set<(nat,nat)>
+  function {:opaque} set_digit(p: Bits, q: Bits, i: nat) : set<(nat,nat)>
   {
     set a:nat, b: nat
           | a <= i && b <= i && a + b == i
@@ -172,6 +172,7 @@ module F2_X_Lemmas {
   lemma mset_mul_F2_X_digit(p: Bits, q: Bits, i: nat)
   ensures mul_F2_X_digit(p, q, i) == parity(set_digit(p, q, i))
   {
+    reveal_set_digit();
     mset_mul_F2_X_digit_partial(p, q, i, 0);
     assert set_digit(p, q, i)
         == set_partial(p, q, i, 0);
@@ -198,11 +199,13 @@ module F2_X_Lemmas {
 
             forall a | a in setA ensures exists b :: b in setB && (a, b) in relation
             {
+              reveal_set_digit();
               var b := (a.1, a.0);
               assert b in setB && (a, b) in relation;
             }
             forall b | b in setB ensures exists a :: a in setA && (a, b) in relation
             {
+              reveal_set_digit();
               var a := (b.1, b.0);
               assert a in setA && (a, b) in relation;
             }
@@ -271,6 +274,7 @@ module F2_X_Lemmas {
           );
           {
             mset_mul_F2_X_digit(p, q, j);
+            reveal_set_digit();
           }
           bool_xor(
             parity(set_digit(p, q, j)),
@@ -295,11 +299,13 @@ module F2_X_Lemmas {
                   var relation := iset a:((nat,nat),(nat,nat,nat)) | a.0.0 == a.1.0 && a.0.1 == a.1.1;
                   forall a | a in setA ensures exists b :: b in setB && (a, b) in relation
                   {
+                    reveal_set_digit();
                     var b := (a.0, a.1, i-j);
                     assert b in setB && (a, b) in relation;
                   }
                   forall b | b in setB ensures exists a :: a in setA && (a, b) in relation
                   {
+                    reveal_set_digit();
                     var a := (b.0, b.1);
                     assert a in setA && (a, b) in relation;
                   }
@@ -380,6 +386,7 @@ module F2_X_Lemmas {
           );
           {
             mset_mul_F2_X_digit(q, r, i-j);
+            reveal_set_digit();
           }
           bool_xor(
             parity(set_digit(q, r, i-j)),
@@ -404,11 +411,13 @@ module F2_X_Lemmas {
                   var relation := iset a:((nat,nat),(nat,nat,nat)) | a.0.0 == a.1.1 && a.0.1 == a.1.2;
                   forall a | a in setA ensures exists b :: b in setB && (a, b) in relation
                   {
+                    reveal_set_digit();
                     var b := (j, a.0, a.1);
                     assert b in setB && (a, b) in relation;
                   }
                   forall b | b in setB ensures exists a :: a in setA && (a, b) in relation
                   {
+                    reveal_set_digit();
                     var a := (b.1, b.2);
                     assert a in setA && (a, b) in relation;
                   }
@@ -498,6 +507,7 @@ module F2_X_Lemmas {
           }
           parity(set_digit(p + zeroes(n), q, i));
           {
+            reveal_set_digit();
             assert set_digit(p + zeroes(n), q, i)
                 == set_digit(p, q, i);
           }
@@ -515,6 +525,7 @@ module F2_X_Lemmas {
           }
           parity(set_digit(p + zeroes(n), q, i));
           {
+            reveal_set_digit();
             assert set_digit(p + zeroes(n), q, i) == {};
             assert |set_digit(p + zeroes(n), q, i)| == 0;
             assert 0 % 2 == 0;
@@ -543,6 +554,7 @@ module F2_X_Lemmas {
     forall i | 0 <= i < |y| ensures !y[i]
     {
       mset_mul_F2_X_digit(a, [], i);
+      reveal_set_digit();
       assert set_digit(a, [], i) == {};
       assert |set_digit(a, [], i)| == 0;
       assert 0 % 2 == 0;
@@ -862,10 +874,17 @@ module F2_X_Lemmas {
   {
     mset_mul_F2_X_digit(x, y, |x| + |y| - 1);
     reveal_parity();
+    reveal_set_digit();
     assert set_digit(x, y, |x| + |y| - 1) == {};
     assert |set_digit(x, y, |x| + |y| - 1)| == 0;
     assert 0 % 2 == 0;
   }
+
+  /*function {:opaque} parity_rev_relation(x: int, y: int) : iset<((nat,nat),(nat,nat))> {
+    iset a:((nat,nat),(nat,nat))
+          | a.0.0 + a.1.0 == x- 1
+          && a.0.1 + a.1.1 == y - 1
+  }*/
 
   lemma parity_rev(x: seq<bool>, y: seq<bool>, i: nat)
   requires i >= 1
@@ -882,6 +901,8 @@ module F2_X_Lemmas {
 
       forall a | a in setA ensures exists b :: b in setB && (a, b) in relation
       {
+        reveal_set_digit();
+        //reveal_parity_rev_relation();
         var b := (|x| - 1 - a.0, |y| - 1 - a.1);
         assert bits_get(reverse(x), b.0) == bits_get(x, a.0);
         assert bits_get(reverse(y), b.1) == bits_get(y, a.1);
@@ -890,13 +911,22 @@ module F2_X_Lemmas {
       }
       forall b | b in setB ensures exists a :: a in setA && (a, b) in relation
       {
+        reveal_set_digit();
+        //reveal_parity_rev_relation();
         var a := (|x| - 1 - b.0, |y| - 1 - b.1);
         assert bits_get(reverse(x), b.0) == bits_get(x, a.0);
         assert bits_get(reverse(y), b.1) == bits_get(y, a.1);
         assert a in setA;
         assert (a, b) in relation;
       }
-      assume false;
+      forall a1, a2, b | a1 in setA && a2 in setA && b in setB && (a1, b) in relation && (a2, b) in relation
+      ensures a1 == a2
+      {
+      }
+      forall a, b1, b2 | b1 in setB && b2 in setB && a in setA && (a, b1) in relation && (a, b2) in relation
+      ensures b1 == b2
+      {
+      }
 
       SetBijectivity.BijectivityImpliesEqualCardinality(setA, setB, relation);
     }
